issues/issue_22.v
@@ -1,0 +1,13 @@
+Require Import Cdcl.Itauto.
+
+Goal forall (P P0 P1 P2 P3 P4 P5 : Prop),
+    P5 ->
+    (P4 -> False) ->
+    P3 ->
+    (P2 -> P3 -> P5 -> P1) ->
+    (P1 -> P0) ->
+    (P3 -> P) -> (P0 -> P1) -> (P0 -> (P2 \/ P /\ P1)) /\ ((P2 \/ P /\ P1) -> P0).
+Proof.
+  intros.
+  itauto idtac.
+Qed.
