issues/issue_23.v
@@ -1,0 +1,28 @@
+Require Import Cdcl.Itauto.
+Require Import List.
+
+Goal forall (P P0 P1: Prop),
+  (P1 -> P0) ->
+  (P0 -> P1) ->
+  ((P0 \/ P -> False) -> (P1 -> False) /\ (P -> False)) /\
+  ((P1 -> False) /\ (P -> False) -> P0 \/ P -> False).
+Proof.
+  intros.
+  itauto idtac.
+Qed.
+
+Goal forall P0 P1 (D:Prop),
+    (((P0 \/ P1 -> False) -> (P1 -> False) /\ (P0 -> False)) -> D) ->
+  D.
+Proof.
+  intros P0 P1 D.
+  itauto idtac.
+Qed.
+
+Goal forall P0 P1 (D:Prop),
+    (((P0 \/ P1 -> False) -> (P1 -> False) /\ (P0 -> False)) -> D) ->
+  D.
+Proof.
+  intros P0 P1 D.
+  itauto idtac.
+Qed.
